test/SDK/MessageHeader.dfy
@@ -13,126 +13,94 @@ module TestMessageHeader {
   import UTF8
   import MessageHeader
   import TestUtils
-
-  method {:test} TestValidKVPair() returns (r: Result<()>) {
-    var keyA, valA := UTF8.Encode("keyA").value, UTF8.Encode("valA").value;
-    var kvPair := (keyA, valA);
-    r := Require(MessageHeader.ValidKVPair(kvPair));
-  }
-
-  method {:test} TestValidKVPairTooLong() returns (r: Result<()>) {
-    var keyA := UTF8.Encode("keyA").value;
-    var invalidVal := seq(0x1_0000, _ => 0);
-    TestUtils.AssumeLongSeqIsValidUTF8(invalidVal);
-    var kvPair := (keyA, invalidVal);
-    r := Require(!MessageHeader.ValidKVPair(kvPair));
-  }
-
-  method {:test} TestKVPairEntriesLength() returns (r: Result<()>) {
-    var keyA, valA := UTF8.Encode("keyA").value, UTF8.Encode("valA").value;
-    var kvPairs := [(keyA, valA)];
-    var len := MessageHeader.KVPairEntriesLength(kvPairs, 0, |kvPairs|);
-
-    r := RequireEqual(len, 2 + |keyA| + 2 + |valA|);
-  }
-
-  method {:test} TestKVPairsLength() returns (r: Result<()>) {
-    var keyA, valA := UTF8.Encode("keyA").value, UTF8.Encode("valA").value;
-    var kvPairs := [(keyA, valA)];
-    var len := MessageHeader.KVPairsLength(kvPairs);
-
-    r := RequireEqual(len, 2 + 2 + |keyA| + 2 + |valA|);
-  }
-
-  method {:test} TestValidAAD() returns (r: Result<()>) {
-    var keyA, valA := UTF8.Encode("keyA").value, UTF8.Encode("valA").value;
-    var kvPairs := [(keyA, valA)];
-    r := Require(MessageHeader.ValidAAD(kvPairs));
-  }
-
-  method {:test} TestValidAADInvalidPairs() returns (r: Result<()>) {
-    var keyA := UTF8.Encode("keyA").value;
-    var invalidVal := seq(0x1_0000, _ => 0);
-    TestUtils.AssumeLongSeqIsValidUTF8(invalidVal);
-    var kvPairs := [(keyA, invalidVal)];
-    r := Require(!MessageHeader.ValidAAD(kvPairs));
-  }
-
-  // TODO test for true if EC is just under serialization size limit of 0x1_0000
-
-  // TODO test for false if EC exceeds serialization size limit of 0x1_0000
   
-  method {:test} TestValidKVPairs() returns (r: Result<()>) {
-    var keyA, valA := UTF8.Encode("keyA").value, UTF8.Encode("valA").value;
-    var kvPairs := [(keyA, valA)];
-    r := Require(MessageHeader.ValidKVPairs(kvPairs));
+  method {:test} TestComputeValidAADEmpty() returns (r: Result<()>) {
+    var kvPairs := [];
+    var valid := MessageHeader.ComputeValidAAD(kvPairs);
+    r := Require(valid);
   }
 
-  method {:test} TestValidKVPairsInvalidPair() returns (r: Result<()>) {
+  method {:test} TestComputeValidAADOnePair() returns (r: Result<()>) {
+    var keyA, valA := UTF8.Encode("keyA").value, UTF8.Encode("valA").value;
+    var kvPairs := [(keyA, valA)];
+    var valid := MessageHeader.ComputeValidAAD(kvPairs);
+    r := Require(valid);
+  }
+
+  method {:test} TestComputeValidAADOnePairMaxSize() returns (r: Result<()>) {
+    var keyA := UTF8.Encode("A").value;
+    // (2^16 - 1) - 2 => 65533 what we want the size of the key value pair to fill
+    // 65533 - 2 - 1 - 2 => 65528 is the size that we want the value to fill
+    var largeVal := seq(65528, _ => 0);
+    var kvPairs :=[(keyA, largeVal)];
+    TestUtils.AssumeLongSeqIsValidUTF8(largeVal);
+    var valid := MessageHeader.ComputeValidAAD(kvPairs);
+    r := Require(valid);
+  }
+
+  method {:test} TestComputeValidAADMaxPairs() returns (r: Result<()>) {
+    var keyA, valA := UTF8.Encode("A").value, UTF8.Encode("A").value;
+    // (2^16 - 1) / (minimum kvPair size) => (2^16 - 1) / 6 => 10922 is the max
+    // number of pairs you can stuff into a valid AAD
+    var kvPairs := seq(10922, _ => (keyA, valA));
+    var valid := MessageHeader.ComputeValidAAD(kvPairs);
+    r := Require(valid);
+  }
+
+  method {:test} TestComputeValidAADTooManyEntries() returns (r: Result<()>) {
+    var keyA, valA := UTF8.Encode("keyA").value, UTF8.Encode("valA").value;
+    var kvPairs := seq(0x1_0000, _ => (keyA, valA));
+    var valid := MessageHeader.ComputeValidAAD(kvPairs);
+    r := Require(!valid);
+  }
+
+  method {:test} TestComputeValidAADTooLarge() returns (r: Result<()>) {
+    var keyA, valA := UTF8.Encode("keyA").value, UTF8.Encode("valA").value;
+    var kvPairs := seq(0x1_FFFF, _ => (keyA, valA));
+    var valid := MessageHeader.ComputeValidAAD(kvPairs);
+    r := Require(!valid);
+  }
+
+  method {:test} TestComputeValidAADPairTooBig() returns (r: Result<()>) {
     var keyA := UTF8.Encode("keyA").value;
     var invalidVal := seq(0x1_0000, _ => 0);
+    var kvPairs :=[(keyA, invalidVal)];
     TestUtils.AssumeLongSeqIsValidUTF8(invalidVal);
-    var kvPairs := [(keyA, invalidVal)];
-    r := Require(!MessageHeader.ValidKVPairs(kvPairs));
+    var valid := MessageHeader.ComputeValidAAD(kvPairs);
+    r := Require(!valid);
   }
 
-  method {:test} TestValidKVPairsUnsorted() returns (r: Result<()>) {
+  method {:test} TestComputeValidAADUnsorted() returns (r: Result<()>) {
     var keyA, valA := UTF8.Encode("keyA").value, UTF8.Encode("valA").value;
     var keyB, valB := UTF8.Encode("keyB").value, UTF8.Encode("valB").value;
     var kvPairs := [(keyB, valB), (keyA, valA)];
-    r := Require(!MessageHeader.ValidKVPairs(kvPairs));
+    var valid := MessageHeader.ComputeValidAAD(kvPairs);
+    r := Require(!valid);
   }
 
-  method {:test} TestSortedKVPairs() returns (r: Result<()>) {
-    var keyA, valA := UTF8.Encode("keyA").value, UTF8.Encode("valA").value;
-    var keyB, valB := UTF8.Encode("keyB").value, UTF8.Encode("valB").value;
-    var kvPairs := [(keyA, valA), (keyB, valB)];
-    r := Require(MessageHeader.SortedKVPairs(kvPairs));
+  method {:test} TestComputeKVPairsLengthEmpty() returns (r: Result<()>) {
+    var kvPairs := [];
+
+    var len := MessageHeader.ComputeKVPairsLength(kvPairs);
+    r := RequireEqual(len as int, 0);
   }
 
-  method {:test} TestSortedKVPairsHasDuplicate() returns (r: Result<()>) {
-    var keyA, valA := UTF8.Encode("keyA").value, UTF8.Encode("valA").value;
-    var kvPairs := [(keyA, valA), (keyA, valA)];
-    r := Require(MessageHeader.SortedKVPairs(kvPairs));
-  }
-
-  method {:test} TestSortedKVPairsEmpty() returns (r: Result<()>) {
-    r := Require(MessageHeader.SortedKVPairs([]));
-  }
-
-  method {:test} TestSortedKVPairsUnsorted() returns (r: Result<()>) {
-    var keyA, valA := UTF8.Encode("keyA").value, UTF8.Encode("valA").value;
-    var keyB, valB := UTF8.Encode("keyB").value, UTF8.Encode("valB").value;
-    var kvPairs := [(keyB, valB), (keyA, valA)];
-    r := Require(!MessageHeader.ValidKVPairs(kvPairs));
-  }
-
-  method {:test} TestKVPairsToSeq() returns (r: Result<()>) {
+  method {:test} TestComputeKVPairsLengthOnePair() returns (r: Result<()>) {
     var keyA, valA := UTF8.Encode("keyA").value, UTF8.Encode("valA").value;
     var kvPairs := [(keyA, valA)];
-    reveal MessageHeader.ValidKVPairs();
-    var expectedBytes := [0, 1, 0, 4, 107, 101, 121, 65, 0, 4, 118, 97, 108, 65];
-    r := RequireEqual(MessageHeader.KVPairsToSeq(kvPairs), expectedBytes);
+
+    var expectedSerialization := [0, 1, 0, 4, 107, 101, 121, 65, 0, 4, 118, 97, 108, 65];
+    var len := MessageHeader.ComputeKVPairsLength(kvPairs);
+    r := RequireEqual(len as int, |expectedSerialization|);
   }
 
-  // TODO: test KVPairsToSeq up to serialization size limit (2^16)
-
-  method {:test} TestKVPairEntriesToSeq() returns (r: Result<()>) {
-    var keyA, valA := UTF8.Encode("keyA").value, UTF8.Encode("valA").value;
-    var keyB, valB := UTF8.Encode("keyB").value, UTF8.Encode("valB").value;
-    var kvPairs := [(keyA, valA), (keyB, valB)];
-    var expectedBytes := [0, 4, 107, 101, 121, 65, 0, 4, 118, 97, 108, 65, 0, 4, 107, 101, 121, 66, 0, 4, 118, 97, 108, 66];
-    r := RequireEqual(MessageHeader.KVPairEntriesToSeq(kvPairs, 0, |kvPairs|), expectedBytes);
+  method {:test} TestComputeKVPairsLengthLong() returns (r: Result<()>) {
+    var keyA := UTF8.Encode("A").value;
+    var largeVal := seq(0x1_0000, _ => 0);
+    TestUtils.AssumeLongSeqIsValidUTF8(largeVal);
+    var kvPairs :=[(keyA, largeVal)];
+    
+    var len := MessageHeader.ComputeKVPairsLength(kvPairs);
+    r := RequireEqual(len as int, 7 + |largeVal|); // 7 bytes needed for kvPairs count, key size, and key
   }
-
-  // TODO: test KVPairEntriesToSeq up to serialization size limit (2^16 - 2)
-
-  method {:test} TestKVPairToSeq() returns (r: Result<()>) {
-    var keyA, valA := UTF8.Encode("keyA").value, UTF8.Encode("valA").value;
-    var kvPair := (keyA, valA);
-    var expectedBytes := [0, 4, 107, 101, 121, 65, 0, 4, 118, 97, 108, 65];
-    r := RequireEqual(MessageHeader.KVPairToSeq(kvPair), expectedBytes);
-  }
-
-  // TODO: test KVPairEntriesToSeq up to serialization size limit (2^16 - 4)
 }
